Update EpistemicLogicActions.lean

EpistemicLogicActions.lean
@@ -23,27 +23,53 @@ notation m₁ " ‖ " m₂ => Message.concat m₁ m₂
 
 inductive Formula (σ : Nat) where
 | atom : Fin σ → Formula σ
+| true : Formula σ 
 | neg : Formula σ → Formula σ
 | implies : Formula σ → Formula σ → Formula σ
 | belief : Agent → Formula σ → Formula σ
 | awareness : Agent → Message σ → Formula σ
 | send : Agent → Agent → Message σ → Formula σ → Formula σ
 | recv : Agent → Message σ → Formula σ → Formula σ
+| gen : Agent → Message σ → Formula σ → Formula σ 
+| fresh : Agent → Message σ → Formula σ 
 deriving Repr, BEq 
 
 notation " #ϕ " i => Formula.atom i
+notation " ⊤ " => Formula.true 
 notation " ~ " φ => Formula.neg φ
-notation φ " ⊃ " ψ => Formula.implies φ ψ
-notation φ " ⋁ " ψ => ((~φ) ⊃ ψ)
+notation " ⊥ " => (~⊤)
+notation φ " implies " ψ => Formula.implies φ ψ
+notation φ " ⋁ " ψ => ((~φ) implies ψ)
 notation φ " ⋀ " ψ => ~((~φ) ⋁ (~ψ))
 notation " 𝔹 " i " , " φ => Formula.belief i φ
 notation " 𝕏 " i " , " m => Formula.awareness i m
+notation " Δ " i " , " m => Formula.fresh i m 
 notation " 𝕂 " i " , " φ => (𝔹 i, φ) ⋀ φ 
 notation " [send " i " , " j " (" μ " )] " φ => Formula.send i j μ φ
 notation " [recv " i " (" μ ")]" φ => Formula.recv i μ φ
+notation " [gen " i " (" μ ")]" φ => Formula.gen i μ φ 
 
-notation φ " ⋁ " ψ => (~φ) ⊃ ψ
-notation φ " ⋀ " ψ => ~((~φ) ⋁ (~ψ))
+def FreshMessage (m : Message σ) (la : List Agent) : Formula σ := 
+  List.foldr (fun p q => p ⋁ q) ⊥ $ List.map (fun ag => (Δ ag, m)) la 
+
+notation "Δ" m "[of " la "]" => FreshMessage m la 
+
+-- def SupremumOverDeltaAgents (m : Message σ) (la : List Agent) : Bool := 
+--   (List.map (fun ag => (Δ ag, m)) la).contains m
+
+-- def SupremumOverDeltaAgentsAsFormula (a : Agent) (m : Message σ) (la : List Agent) : Formula σ :=
+--   if SupremumOverDeltaAgents a m la then φ else (~φ)
+
+notation " 𝔼 " i "[of " li "]" m => (𝕏 i, m) ⋀ (Δ m [of li])
+
+variable { τ : Nat }
+variable { m : Message σ }
+def la : List Agent := [ "Alice", "Bob" ]
+#check 𝔼 "Alice" [of la] m
+
+
+-- notation φ " ⋁ " ψ => (~φ) implies ψ
+-- notation φ " ⋀ " ψ => ~((~φ) ⋁ (~ψ))
 
 /-
   **Proof system**
@@ -52,19 +78,30 @@ notation φ " ⋀ " ψ => ~((~φ) ⋁ (~ψ))
 def Context (σ : Nat) := List $ Formula σ
 
 inductive Proof {σ : Nat} : Context σ → Formula σ → Prop  
-| ax { Γ } { p : Formula σ } (h : Γ.contains p) : Proof Γ p 
-| pl₁ { Γ } { p q : Formula σ } : Proof Γ (p ⊃ (q ⊃ p))
-| pl₂ { Γ } { p q r : Formula σ } : Proof Γ $ (p ⊃ (q ⊃ r)) ⊃ ((p ⊃ q) ⊃ (p ⊃ r)) 
-| pl₃ { Γ } { p q : Formula σ } : Proof Γ $ ((~p) ⊃ ~q) ⊃ (((~p) ⊃ q) ⊃ p)
-| KαSend { Γ } { φ ψ : Formula σ } {a b : Agent} { m : Message σ } : Proof Γ $ ([send a,b(m)](φ ⊃ ψ)) ⊃ (([send a,b(m)]φ) ⊃ ([send a,b(m)]ψ))
-| KαRecv { Γ } { φ ψ : Formula σ } {b : Agent} { m : Message σ } : Proof Γ $ ([recv b(m)](φ ⊃ ψ)) ⊃ (([recv b(m)]φ) ⊃ ([recv b(m)]ψ))
-| K𝔹 { Γ } { φ ψ : Formula σ } {a : Agent} : Proof Γ $ (𝔹 a, (φ ⊃ ψ)) ⊃ ((𝔹 a, φ) ⊃ (𝔹 a, ψ))
-| D { Γ } { φ : Formula σ } {a : Agent} : Proof Γ $ (𝔹 a, φ) ⊃ ~(𝔹 a, (~φ))
-| _4 { Γ } { φ : Formula σ } {a : Agent} : Proof Γ $ (𝔹 a, φ) ⊃ (𝔹 a, (𝔹 a, φ)) 
-| _5 { Γ } { φ : Formula σ } {a : Agent} : Proof Γ $ (~(𝔹 a, φ)) ⊃ (𝔹 a, (~(𝔹 a, φ))) 
+| ax { Γ } { p : Formula σ } (h : Γ.Mem p) : Proof Γ p 
+| pl₁ { Γ } { p q : Formula σ } : Proof Γ (p implies (q implies p))
+| pl₂ { Γ } { p q r : Formula σ } : Proof Γ $ (p implies (q implies r)) implies ((p implies q) implies (p implies r)) 
+| pl₃ { Γ } { p q : Formula σ } : Proof Γ $ ((~p) implies ~q) implies (((~p) implies q) implies p)
+| KαSend { Γ } { φ ψ : Formula σ } {a b : Agent} { m : Message σ } : Proof Γ $ ([send a,b(m)](φ implies ψ)) implies (([send a,b(m)]φ) implies ([send a,b(m)]ψ))
+| KαRecv { Γ } { φ ψ : Formula σ } {b : Agent} { m : Message σ } : Proof Γ $ ([recv b(m)](φ implies ψ)) implies (([recv b(m)]φ) implies ([recv b(m)]ψ))
+| K𝔹 { Γ } { φ ψ : Formula σ } {a : Agent} : Proof Γ $ (𝔹 a, (φ implies ψ)) implies ((𝔹 a, φ) implies (𝔹 a, ψ))
+| D { Γ } { φ : Formula σ } {a : Agent} : Proof Γ $ (𝔹 a, φ) implies ~(𝔹 a, (~φ))
+| _4 { Γ } { φ : Formula σ } {a : Agent} : Proof Γ $ (𝔹 a, φ) implies (𝔹 a, (𝔹 a, φ)) 
+| _5 { Γ } { φ : Formula σ } {a : Agent} : Proof Γ $ (~(𝔹 a, φ)) implies (𝔹 a, (~(𝔹 a, φ))) 
 --
-| MP { Γ } { p q : Formula σ } (hpq : Proof Γ $ p ⊃ q) (hp : Proof Γ p) : Proof Γ q
+| MP { Γ } { p q : Formula σ } (hpq : Proof Γ $ p implies q) (hp : Proof Γ p) : Proof Γ q
 | NECB { Γ } { φ : Formula σ } {a : Agent} (hφ : Proof Γ φ) : Proof Γ $ 𝔹 a, φ 
+| NECSend { Γ } {φ : Formula σ} {a b : Agent} {m : Message σ} (hφ : Proof Γ φ) : Proof Γ $ [send a,b(m)]φ 
+--
+| FreshConst { Γ } {a : Agent} {m : Message σ} : Proof Γ $ (Δ a, m) implies (𝕏 a, m)
+-- Natural Deduction
+| AndLeft { Γ } {a : Agent} {φ ψ : Formula σ} (h : Proof Γ $ φ ⋀ ψ) : Proof Γ φ  
+| AndRight { Γ } {a : Agent} {φ ψ : Formula σ} (h : Proof Γ $ φ ⋀ ψ) : Proof Γ ψ 
+| AndIntro { Γ } {a : Agent} {φ ψ : Formula σ} (h₁ : Proof Γ $ φ) (h₂ : Proof Γ $ ψ) : Proof Γ $ φ ⋀ ψ 
+| BDistOverConj { Γ } {a : Agent} {φ ψ : Formula σ} (h₁ : Proof Γ $ (𝔹 a, φ)) (h₂ : Proof Γ $ (𝔹 a, ψ)) : Proof Γ $ (𝔹 a, (φ ⋀ ψ))
+| BDistFromConj_left { Γ } {a : Agent} {φ ψ : Formula σ} (h : Proof Γ $ 𝔹 a, (φ ⋀ ψ)) : Proof Γ $ 𝔹 a, φ 
+| BDistFromConj_right { Γ } {a : Agent} {φ ψ : Formula σ} (h : Proof Γ $ 𝔹 a, (φ ⋀ ψ)) : Proof Γ $ 𝔹 a, ψ
+| BMP { Γ } {a : Agent} {φ ψ : Formula σ} (h₀ : Proof Γ $ 𝔹 a, (φ implies ψ)) (h₁ : Proof Γ $ 𝔹 a, φ) : Proof Γ $ 𝔹 a, ψ 
 
 notation Γ " ⊢ " φ => Proof Γ φ 
 
@@ -75,22 +112,28 @@ structure Model (σ : Nat) :=
   R𝔹 : Agent → World σ → World σ → Bool 
   RPDLSend : Agent → Agent → Message σ → World σ → World σ → Bool 
   RPDLRecv : Agent → Message σ → World σ → World σ → Bool
+  RPDLGen : Agent → Message σ → World σ → World σ → Bool 
   Valuation : Fin σ → World σ → Bool
   ValuationConstants : Agent → Message σ → World σ → Bool    
+  ValuationFresh : Agent → Message σ → World σ → Bool 
   BSerial : ∀ (a : Agent) (x : World σ), ∃ (y : World σ), R𝔹 a x y 
   BTrans : ∀ (a : Agent) (x : World σ) (y : World σ) (z : World σ), ((R𝔹 a x y ∧ R𝔹 a y z) → R𝔹 a x z)  
-  BEuclid : ∀ (a : Agent) (x : World σ) (y : World σ) (z : World σ), ((R𝔹 a x y ∧ R𝔹 a x z) → R𝔹 a y z) 
+  BEuclid : ∀ (a : Agent) (x : World σ) (y : World σ) (z : World σ), ((R𝔹 a x y ∧ R𝔹 a x z) → R𝔹 a y z)
+  FreshIsConstant : ∀ (a : Agent) (m : Message σ) (x : World σ), ((ValuationFresh a m x) → (ValuationConstants a m x))
   
 @[simp]
 def ModelSatisfiesInState {σ : Nat} (M : Model σ) (w : World σ) (φ : Formula σ) : Prop := 
   match φ with 
   | Formula.atom p => Model.Valuation M p w   
-  | 𝕏 a, m => Model.ValuationConstants M a m w 
+  | Formula.true => True 
+  | 𝕏 a, m => Model.ValuationConstants M a m w
+  | Δ a, m => Model.ValuationFresh M a m w 
   | ~φ => ¬ (ModelSatisfiesInState M w φ)
-  | φ ⊃ ψ => (ModelSatisfiesInState M w φ) → (ModelSatisfiesInState M w ψ)
+  | (φ implies ψ) => (ModelSatisfiesInState M w φ) → (ModelSatisfiesInState M w ψ)
   | 𝔹 a, φ => ∀ (v : World σ), ((Model.R𝔹 M a w v) → (ModelSatisfiesInState M v φ)) 
   | [send a,b(m)] φ => ∀ (v : World σ), ((Model.RPDLSend M a b m w v) → (ModelSatisfiesInState M v φ))
   | [recv b(m)] φ => ∀ (v : World σ), ((Model.RPDLRecv M b m w v) → (ModelSatisfiesInState M v φ))
+  | [gen a(m)] φ => ∀ (v : World σ), (Model.RPDLGen M a m w v) → (ModelSatisfiesInState M v φ)
   
 
 def List.subsetOf {α : Type} [BEq α] (l₀ : List α) (l₁ : List α) : Bool := 
@@ -106,15 +149,15 @@ instance : BEq $ World σ where
 
 @[simp]
 def ModelSatisfies {σ : Nat} (M : Model σ) (φ : Formula σ) := 
-  ∀ (w : World σ), M.Worlds.contains w →  ModelSatisfiesInState M w φ 
+  ∀ (w : World σ), M.Worlds.Mem w →  ModelSatisfiesInState M w φ 
 
 @[simp]
 def ModelSatisfiesContext {σ : Nat} (M : Model σ) (Γ : Context σ) : World σ → Prop := 
-  fun (w : World σ) => ∀ (φ : Formula σ), ((Γ.contains φ) → (ModelSatisfiesInState M w φ))
+  fun (w : World σ) => ∀ (φ : Formula σ), ((Γ.Mem φ) → (ModelSatisfiesInState M w φ))
 
 @[reducible]
 inductive SemanticCsq {σ : Nat} (Γ : Context σ) (φ : Formula σ) : Prop :=
-  | is_true (m : ∀ (M : Model σ) (w : World σ), (M.Worlds.contains w) → ((ModelSatisfiesContext M Γ w) → ModelSatisfiesInState M w φ)) 
+  | is_true (m : ∀ (M : Model σ) (w : World σ), (M.Worlds.Mem w) → ((ModelSatisfiesContext M Γ w) → ModelSatisfiesInState M w φ)) 
 
 notation Γ " ⊧₀ " φ => SemanticCsq Γ φ 
 
@@ -129,87 +172,313 @@ theorem currying_uncurrying { p q : Prop } : (p ∧ q → r) ↔ (p → q → r)
   . intros h₁ h₂ 
     exact (h₁ $ And.left h₂) $ And.right h₂ 
 
-@[simp]
-theorem forward {α : Type} {p : α → Prop} {y : α} (h : ∀ x, (p y → p x)) : p y → ∀ x, p x := by 
-  intro py 
-  intro x 
-  apply h
-  exact py 
+-- @[simp]
+-- theorem forward {α : Type} {p : α → Prop} {y : α} (h : ∀ x, (p y → p x)) : p y → ∀ x, p x := by 
+--   intro py 
+--   intro x 
+--   apply h
+--   exact py 
 
-@[simp]
-theorem backward {a : Type} {p : α → Prop} {y : α} (h : p y → ∀ x, p x) : ∀ x, (p y → p x) := by 
-  intros x py 
-  apply (h py)   
+-- @[simp]
+-- theorem backward {a : Type} {p : α → Prop} {y : α} (h : p y → ∀ x, p x) : ∀ x, (p y → p x) := by 
+--   intros x py 
+--   apply (h py)   
 
--- theorem Soundness {σ : Nat} (Γ : Context σ) (φ : Formula σ) : (Γ ⊢ φ) → (Γ ⊧₀ φ) := by 
---   intros h
---   induction h 
---   case ax ψ h₀ => 
---     apply SemanticCsq.is_true; intros M w _ h₂; dsimp at h₂ 
---     specialize h₂ ψ; exact h₂ h₀ 
---   case pl₁ p q =>
---     apply SemanticCsq.is_true; intros M w _ h₂; dsimp at h₂ 
---     dsimp at *; specialize h₂ p; intros h₃ _; exact h₃ 
---   case pl₂ p q r => 
---     apply SemanticCsq.is_true; intros M w _ _ ; dsimp at *
---     intros h₃ h₄ h₅; exact (h₃ h₅) (h₄ h₅) 
---   case pl₃ p q => 
---     apply SemanticCsq.is_true; intros M w _ _ ; dsimp at * 
---     intros h₃ h₄; apply byContradiction (fun (hp : ¬ModelSatisfiesInState M w p) => 
---       let h₅ := h₃ hp ; let h₆ := h₄ hp ; show False from h₅ h₆)
---   case KαSend φ ψ a b m => 
---     apply SemanticCsq.is_true; intros M w _ _; dsimp at * 
---     intros h₂ h₃ v; specialize h₂ v; specialize h₃ v 
---     intro h₄; exact (h₂ h₄) (h₃ h₄) 
---   case KαRecv φ ψ b m => 
---     apply SemanticCsq.is_true; intros M w _ _; dsimp at * 
---     intros h₂ h₃ v; specialize h₂ v; specialize h₃ v 
---     intro h₄; exact (h₂ h₄) (h₃ h₄) 
---   case K𝔹 φ ψ a => 
---     apply SemanticCsq.is_true; intros M w _ _; dsimp at * 
---     intros h₂ h₃ v; specialize h₂ v; specialize h₃ v 
---     intro h₄; exact (h₂ h₄) (h₃ h₄)
---   case D φ a => 
---     apply SemanticCsq.is_true; intros M w _ _; 
---     intros h₀ h₁
---     dsimp at * 
---     let hEuclid := M.BEuclid a w w w 
---     sorry 
---   case _4 φ a => 
---     apply SemanticCsq.is_true; intros M w _ _; dsimp at * 
---     intros h₀ u h₂ v h₃; specialize h₀ v 
---     let hTrans := M.BTrans a w u v; simp at hTrans 
---     exact h₀ $ (hTrans h₂) h₃ 
---   case _5 φ a => 
---     apply SemanticCsq.is_true; intros M w _ _; dsimp at * 
---     intros h₀ u h₁ h₂
---     let hTrans := M.BTrans a w u 
---     simp [*] at hTrans 
---     let hAnd := And.intro h₁ h₂ 
---     simp [*] at hAnd 
---     sorry 
---   case MP p q h₂ h₃ h₄ h₅ =>
---     apply SemanticCsq.is_true; intros M w th₀ th₁ 
---     have hmp := Proof.MP h₂ h₃ 
---     have hSound := Soundness Γ q 
---     have hq := hSound hmp 
---     induction hq with 
---     | is_true ih => 
---       specialize ih M w 
---       exact (ih th₀) th₁ 
---   case NECB p a h₀ h₁ =>
---     apply SemanticCsq.is_true; intros M w th₀ th₁ 
---     dsimp at * 
---     specialize th₁ p 
---     intros v hv 
---     sorry 
+theorem Soundness {σ : Nat} (Γ : Context σ) (φ : Formula σ) : (Γ ⊢ φ) → (Γ ⊧₀ φ) := by 
+  intros h
+  induction h 
+  case ax ψ h₀ => 
+    apply SemanticCsq.is_true; intros M w _ h₂; dsimp at h₂ 
+    specialize h₂ ψ; 
+    exact h₂ h₀ 
+  case pl₁ p q =>
+    apply SemanticCsq.is_true; intros M w _ h₂; dsimp at h₂ 
+    dsimp at *; specialize h₂ p; intros h₃ _; exact h₃ 
+  case pl₂ p q r => 
+    apply SemanticCsq.is_true; intros M w _ _ ; dsimp at *
+    intros h₃ h₄ h₅; exact (h₃ h₅) (h₄ h₅) 
+  case pl₃ p q => 
+    apply SemanticCsq.is_true; intros M w _ _ ; dsimp at * 
+    intros h₃ h₄; apply byContradiction (fun (hp : ¬ModelSatisfiesInState M w p) => 
+      let h₅ := h₃ hp ; let h₆ := h₄ hp ; show False from h₅ h₆)
+  case KαSend φ ψ a b m => 
+    apply SemanticCsq.is_true; intros M w _ _; dsimp at * 
+    intros h₂ h₃ v; specialize h₂ v; specialize h₃ v 
+    intro h₄; exact (h₂ h₄) (h₃ h₄) 
+  case KαRecv φ ψ b m => 
+    apply SemanticCsq.is_true; intros M w _ _; dsimp at * 
+    intros h₂ h₃ v; specialize h₂ v; specialize h₃ v 
+    intro h₄; exact (h₂ h₄) (h₃ h₄) 
+  case K𝔹 φ ψ a => 
+    apply SemanticCsq.is_true; intros M w _ _; dsimp at * 
+    intros h₂ h₃ v; specialize h₂ v; specialize h₃ v 
+    intro h₄; exact (h₂ h₄) (h₃ h₄)
+  case D φ a => 
+    apply SemanticCsq.is_true; intros M w _ _; 
+    intros h₀ h₁
+    dsimp at * 
+    let hSerial := M.BSerial a w
+    apply Exists.elim hSerial 
+    intro v 
+    specialize h₀ v 
+    specialize h₁ v 
+    intro wRBv
+    have := h₀ wRBv
+    have := h₁ wRBv
+    contradiction 
+  case _4 φ a => 
+    apply SemanticCsq.is_true; intros M w _ _; dsimp at * 
+    intros h₀ u h₂ v h₃; specialize h₀ v 
+    let hTrans := M.BTrans a w u v; simp at hTrans 
+    exact h₀ $ (hTrans h₂) h₃ 
+  case _5 φ a => 
+    apply SemanticCsq.is_true; intros M w _ _ 
+    dsimp at * 
+    intros h₀ u h₁ h₂
+    let hEuclid := M.BEuclid a w u 
+    simp [*] at h₀ 
+    apply Exists.elim h₀ 
+    intro t 
+    specialize h₂ t 
+    specialize hEuclid t 
+    intro h₃ 
+    have h₄ := And.left h₃ 
+    have h₅ := And.intro h₁ h₄ 
+    have h₆ := hEuclid h₅ 
+    have h₇ := h₂ h₆ 
+    have h₈ := And.right h₃ 
+    contradiction 
+  case MP p q h₂ h₃ h₄ h₅ =>
+    apply SemanticCsq.is_true
+    intros M w wmem ctt 
+    cases h₄ with | is_true h₆ => 
+    cases h₅ with | is_true h₇ =>
+    specialize h₆ M w 
+    specialize h₇ M w 
+    let h₈ := (h₆ wmem) ctt 
+    let h₉ := (h₇ wmem) ctt 
+    dsimp at h₈ 
+    exact h₈ h₉ 
+  case NECB p a h₀ h₁ =>
+    apply SemanticCsq.is_true
+    intros M w mem ctt 
+    intros v rel 
+    cases h₁ with | is_true h₂ =>
+    specialize h₂ M w mem ctt 
+    have h := @SemanticCsq.is_true σ Γ (𝔹 a, φ)
+    sorry 
+  case NECSend p q r a h₀ h₁ => 
+    apply SemanticCsq.is_true 
+    intros M w mem ctt 
+    intros v rel 
+    simp [*] at * 
+    specialize ctt p 
+    cases h₁ with | is_true h₂ =>
+    specialize h₂ M w mem 
+    have ax := @Proof.ax σ Γ p 
+    sorry 
+  case FreshConst a m => 
+    apply SemanticCsq.is_true 
+    intros M w _ _ 
+    dsimp at * 
+    exact (M.FreshIsConstant a m w) 
+  case AndLeft a p q h₀ h₁ => 
+    apply SemanticCsq.is_true 
+    intros M w mem ctt 
+    cases h₁ with | is_true h₃ => 
+    skip 
+    specialize h₃ M w mem ctt 
+    simp [*] at * 
+    exact And.left h₃ 
+  case AndRight a p q h₀ h₁ => 
+    apply SemanticCsq.is_true 
+    intros M w mem ctt 
+    cases h₁ with | is_true h₃ => 
+    specialize h₃ M w mem ctt 
+    simp [*] at * 
+    exact And.right h₃ 
+  case AndIntro a p q h₀ h₁ h₂ => 
+    apply SemanticCsq.is_true 
+    intros M w mem ctt 
+    cases h₁ with | is_true h₃ => 
+    cases h₂ with | is_true h₄ => 
+    specialize h₃ M w mem ctt 
+    specialize h₄ M w mem ctt 
+    simp 
+    trivial 
+  case BDistOverConj a p q r h₀ h₁ h₂ =>
+    apply SemanticCsq.is_true 
+    intros M w mem ctt 
+    cases h₁ with | is_true h₃ =>
+    cases h₂ with | is_true h₄ =>
+    specialize h₃ M w mem ctt 
+    specialize h₄ M w mem ctt 
+    simp 
+    intro v 
+    dsimp at h₃ 
+    dsimp at h₄ 
+    specialize h₃ v 
+    specialize h₄ v 
+    intro rel 
+    have h₅ := h₃ rel 
+    have h₆ := h₄ rel 
+    trivial 
+  case BDistFromConj_left _ a p r h₀ h₁ => 
+    apply SemanticCsq.is_true 
+    intros M w mem ctt 
+    cases h₁ with | is_true h₂ =>
+    specialize h₂ M w mem ctt 
+    simp [*] at * 
+    intro v rel 
+    specialize h₂ v
+    have h₃ := h₂ rel 
+    exact And.left h₃   
+  case BDistFromConj_right _ a p r h₀ h₁ => 
+    apply SemanticCsq.is_true 
+    intros M w mem ctt 
+    cases h₁ with | is_true h₂ =>
+    specialize h₂ M w mem ctt 
+    simp [*] at * 
+    intro v rel 
+    specialize h₂ v
+    have h₃ := h₂ rel 
+    exact And.right h₃   
+  case BMP _ a p r h₀ h₁ h₂ => 
+    apply SemanticCsq.is_true 
+    intros M w mem ctt 
+    cases h₁ with | is_true h₃ =>
+    cases h₂ with | is_true h₄ =>
+    specialize h₃ M w mem ctt 
+    specialize h₄ M w mem ctt 
+    simp [*] at * 
+    intro v rel 
+    specialize h₃ v
+    specialize h₄ v 
+    have h₅ := h₃ rel
+    have h₆ := h₄ rel 
+    exact h₅ h₆ 
 
 
+/-
+  **Structural Rules for explicit knowledge**
+-/
+
+open Formula 
+open Proof 
+
+variable {a b b₁ b₂ : Agent}
+variable {m m₁ m₂ k : Message σ}
+variable {Γ : Context σ}
 
 
+def X₁_1 : Formula σ := (𝕏 a, (m₁.concat m₂)) implies ((𝕏 a, m₁) ⋀ (𝕏 a, m₂))
+def X₁_2 : Formula σ := ((𝕏 a, m₁) ⋀ (𝕏 a, m₂)) implies (𝕏 a, (m₁.concat m₂))
+def X₂_1 : Formula σ := (𝕏 a, (Message.symmetricKey a b k)) implies (𝕏 b, (Message.symmetricKey b a k))
+def X₂_2 : Formula σ := (𝕏 b, (Message.symmetricKey b a k)) implies (𝕏 a, (Message.symmetricKey a b k))
+def X₃ : Formula σ := ((𝕏 a, ⦃|m|⦄ pk(b)) ⋀ (𝕏 a, sk(b))) implies (𝕏 a, m)
+def X₄ : Formula σ := ((𝕏 a, ⦃|m|⦄ sk(b)) ⋀ (𝕏 a, pk(b))) implies (𝕏 a, m)
+def X₅ : Formula σ := ((𝕏 a, m₁) ⋀ (𝕏 a, m₂)) implies 𝕏 a, ⦃|m₁|⦄m₂ 
+def X₆ : Formula σ := ((𝕏 a, ⦃|m|⦄ (Message.symmetricKey a b k)) ⋀ (𝕏 a, (Message.symmetricKey a b k))) implies (𝕏 a, m)
+def X₇ : Formula σ := (𝕏 a, ag(a))
 
-#check ModelSatisfiesInState
+/-
+  **General Axioms for actions**
+-/
 
+variable {φ : Formula σ}
+
+def H₀ : Formula σ := ([send b,a(m)]φ) implies ([recv a(m)]φ)
+def H₁ : Formula σ := ([send b,a(m)] φ) implies (𝕏 b, m)
+def H₂ : Formula σ := ([recv a(m)]φ) implies (𝕏 a, m)
+def H₂' : Formula σ := ([recv a(⦃|m|⦄ (Message.symmetricKey a b k))]φ) implies (𝕏 a, ⦃|m|⦄ (Message.symmetricKey a b k))
+
+def H₅ : Formula σ := (([recv a(⦃|m|⦄ (Message.symmetricKey a b k))]φ) ⋀ (𝔹 a, (𝕏 a, m))) implies 𝔹 a, ([send b,a(m)]φ)
+
+/-
+  **Secret key axiom**
+-/
+
+def SK : Formula σ := (𝕏 a, (Message.symmetricKey a b k)) ⋀ (𝕏 b, (Message.symmetricKey a b k))
+
+/-
+  **BAN Logic Theory**
+-/
+
+open Formula 
+open Proof 
+
+variable {a b : Agent}
+variable {m : Message σ}
+variable {φ : Formula σ}
+variable {Γ : Context σ}
+
+def H₀B : Formula σ := (([send b,a(m)] φ) ⋀ (Δ m [of [a, b]])) implies ([recv a(m)] φ)
+def H₃B : Formula σ := ([gen b(m)]φ) implies ((Δ m [of [a,b]]))
+
+
+def BANTheory : Context σ := 
+[
+  @H₀B σ a b m φ, 
+  @H₁ σ a b m φ, 
+  @H₂ σ a m φ,
+  @H₂' σ a b m k φ,
+  @H₃B σ a b m φ,
+  @H₅ σ a b m k φ,
+  @SK σ a b k,
+  @X₁_1 σ a m₁ m₂,
+  @X₆ σ a b m k
+] 
+
+theorem NV {a b : Agent} { m : Message σ } : 
+      ((@BANTheory σ m₁ m₂ k a b m φ) ⊢ 𝔹 a, (Δ m [of [a, b]])) 
+    → ((@BANTheory σ m₁ m₂ k a b m φ) ⊢ (𝔹 a, ([send b, a(m)]φ))) 
+    → ((@BANTheory σ m₁ m₂ k a b m φ) ⊢ (𝔹 a, (𝔼 b [of [a,b]] m))) := by 
+  intros h₁ h₂  
+  have h₁t  : (@BANTheory σ m₁ m₂ k a b m φ) ⊢ ([send b,a(m)] φ) implies (𝕏 b, m) := by repeat constructor 
+  have h₁tn : (@BANTheory σ m₁ m₂ k a b m φ) ⊢ 𝔹 a, (([send b,a(m)] φ) implies (𝕏 b, m)) := NECB h₁t 
+  have h₁₉  : (@BANTheory σ m₁ m₂ k a b m φ) ⊢ 𝔹 a, (𝕏 b, m) := BMP h₁tn h₂ 
+  have h₂₀  : (@BANTheory σ m₁ m₂ k a b m φ) ⊢ 𝔹 a, ((𝕏 b, m) ⋀ (Δ m [of [a, b]])) := BDistOverConj h₁₉ h₁
+  have h₂₁  : (@BANTheory σ m₁ m₂ k a b m φ) ⊢ 𝔹 a, 𝔼 b [of [a, b]] m := h₂₀ 
+  exact h₂₁  
+
+def JR : Formula σ := (𝔹 a, ([gen b(m)]φ)) ⋀ (𝔹 a, (𝔼 b [of [a, b]] m)) implies (𝔼 a [of [a, b]] m)
+
+theorem JR_with_assumptions {a b : Agent} {m : Message σ } : 
+    ((@BANTheory σ m₁ m₂ k a b m φ) ⊢ 𝔹 a, ([gen b(m)]φ))
+  → ((@BANTheory σ m₁ m₂ k a b m φ) ⊢ 𝔹 a, (𝔼 b [of [a, b]] m))
+  → ((@BANTheory σ m₁ m₂ k a b m φ) ⊢ [recv a(m)]φ)
+  → ((@BANTheory σ m₁ m₂ k a b m φ) ⊢ 𝔹 a, (𝔼 a [of [a, b]] m)) := by 
+  intros h₀ _ h₃ 
+  have h₃b  : (@BANTheory σ m₁ m₂ k a b m φ) ⊢ ([gen b(m)]φ) implies ((Δ m [of [a,b]])) := by repeat constructor 
+  have h₃bn : (@BANTheory σ m₁ m₂ k a b m φ) ⊢ 𝔹 a, (([gen b(m)]φ) implies ((Δ m [of [a,b]]))) := NECB h₃b 
+  have h₂   : (@BANTheory σ m₁ m₂ k a b m φ) ⊢ 𝔹 a, (Δ m [of [a,b]]) := BMP h₃bn h₀ 
+  have h₁t  : (@BANTheory σ m₁ m₂ k a b m φ) ⊢ ([recv a(m)]φ) implies (𝕏 a, m) := by repeat constructor 
+  have h₃   : (@BANTheory σ m₁ m₂ k a b m φ) ⊢ 𝕏 a, m := MP h₁t h₃ 
+  have h₃n  : (@BANTheory σ m₁ m₂ k a b m φ) ⊢ 𝔹 a, (𝕏 a, m) := NECB h₃ 
+  have h₄   : (@BANTheory σ m₁ m₂ k a b m φ) ⊢ 𝔹 a, ((𝕏 a, m) ⋀ (Δ m [of [a,b]])) := BDistOverConj h₃n h₂ 
+  have h₅   : (@BANTheory σ m₁ m₂ k a b m φ) ⊢ 𝔹 a, (𝔼 a [of [a, b]] m) := h₄ 
+  exact h₅ 
+
+
+theorem MMSK {a b : Agent} {m k : Message σ} :
+    ((@BANTheory σ m₁ m₂ k a b m φ) ⊢ [recv a(⦃|m|⦄ (Message.symmetricKey a b k))]φ)
+  → ((@BANTheory σ m₁ m₂ k a b m φ) ⊢ 𝔹 a, ([send b,a(m)]φ)) := by 
+  intros h₀ 
+  have h₁   : (@BANTheory σ m₁ m₂ k a b m φ) ⊢ ([recv a(⦃|m|⦄ (Message.symmetricKey a b k))]φ) implies 𝕏 a, ⦃|m|⦄ (Message.symmetricKey a b k) := by repeat constructor 
+  have h₁n  : (@BANTheory σ m₁ m₂ k a b m φ) ⊢ 𝔹 a, (([recv a(⦃|m|⦄ (Message.symmetricKey a b k))]φ) implies 𝕏 a, ⦃|m|⦄ (Message.symmetricKey a b k)) := NECB h₁ 
+  have h₂   : (@BANTheory σ m₁ m₂ k a b m φ) ⊢ (𝔹 a, ([recv a(⦃|m|⦄ (Message.symmetricKey a b k))]φ)) implies 𝔹 a, (𝕏 a, ⦃|m|⦄ (Message.symmetricKey a b k)) := MP K𝔹 h₁n 
+  have h₃   : (@BANTheory σ m₁ m₂ k a b m φ) ⊢  𝔹 a, (𝕏 a, ⦃|m|⦄ (Message.symmetricKey a b k)) := MP h₂ (NECB h₀)
+  have sk   : (@BANTheory σ m₁ m₂ k a b m φ) ⊢ (𝕏 a, (Message.symmetricKey a b k)) ⋀ (𝕏 b, (Message.symmetricKey a b k)) := by repeat constructor 
+  have hskb : (@BANTheory σ m₁ m₂ k a b m φ) ⊢ 𝔹 a, (𝕏 a, (Message.symmetricKey a b k)) := NECB $ @AndLeft σ (@BANTheory σ m₁ m₂ k a b m φ) a (𝕏 a, (Message.symmetricKey a b k)) (𝕏 b, (Message.symmetricKey a b k)) sk
+  have h₄   : (@BANTheory σ m₁ m₂ k a b m φ) ⊢ 𝔹 a, ((𝕏 a, ⦃|m|⦄ (Message.symmetricKey a b k)) ⋀ (𝕏 a, (Message.symmetricKey a b k))) := BDistOverConj h₃ hskb 
+  have x₆   : (@BANTheory σ m₁ m₂ k a b m φ) ⊢ ((𝕏 a, ⦃|m|⦄ (Message.symmetricKey a b k)) ⋀ (𝕏 a, (Message.symmetricKey a b k))) implies (𝕏 a, m) := by repeat constructor 
+  have h₅   : (@BANTheory σ m₁ m₂ k a b m φ) ⊢ 𝔹 a, (𝕏 a, m) := MP (MP K𝔹 (NECB x₆)) h₄ 
+  have h₆   : (@BANTheory σ m₁ m₂ k a b m φ) ⊢ (([recv a(⦃|m|⦄ (Message.symmetricKey a b k))]φ) ⋀ (𝔹 a, (𝕏 a, m))) implies 𝔹 a, ([send b,a(m)]φ) := by repeat constructor 
+  exact MP h₆ (@AndIntro σ (@BANTheory σ m₁ m₂ k a b m φ) a ([recv a(⦃|m|⦄ (Message.symmetricKey a b k))]φ) (𝔹 a, (𝕏 a, m)) h₀ h₅)
+
+
+def SC₁ : Formula σ := 𝔹 a, ([send b, a(m₁.concat m₂)]φ) implies (𝔹 a, [send b,a(m₁)]φ)
+def SC₂ : Formula σ := ([recv a(m₁.concat m₂)]φ) implies ([recv a(m₁)]φ)
 /-
   **Generated model section**
 -/
@@ -227,6 +496,7 @@ structure AutomaticallyGeneratedModel (σ : Nat) :=
   R𝔹 : List $ (Agent × List Nat)
   RPDLSend : List $ (Agent × Agent × Message σ × List Nat)
   RPDLRecv : List $ (Agent × Message σ × List Nat)
+  RPDLGen : List $ (Agent × Message σ × List Nat)
 
 def List.getAtIndex {α : Type} (list : List α) (i : Nat) : Option α :=
   match i with
@@ -239,8 +509,6 @@ def List.getAtIndex! {α : Type} (list : List α) (i : Nat) (default : α) : α 
   | some result => result
 
 def MessageContext (σ : Nat) := List $ Message σ
-
-
 
 def DeductionClosureStep {σ : Nat} (Γ : MessageContext σ) (Γc : MessageContext σ) : MessageContext σ :=
   match Γ with 
@@ -294,18 +562,23 @@ def AwarenessSatisfies {σ : Nat} (M : AutomaticallyGeneratedModel σ) (wIndex :
   let currentAgentState := currentState.getAtIndex! agentStatePosition []
   currentAgentState ⊢μ m 
 
-def ModalKBStates {σ : Nat} (M : AutomaticallyGeneratedModel σ) (wIndex : Nat) (agent : Agent) (relation : List $ (Agent × List Nat)) : List Nat :=
+def ModalKBStates {σ : Nat} (_ : AutomaticallyGeneratedModel σ) (wIndex : Nat) (agent : Agent) (relation : List $ (Agent × List Nat)) : List Nat :=
   let agentRelation : List $ List Nat := ((relation.filter (fun (ag, _) => ag == agent)).map (fun (_, y) => y)).filter (fun list => list.getAtIndex! 0 0 == wIndex)
   let accessibleStates : List Nat := agentRelation.map (fun list => list.getAtIndex! 1 0)
   accessibleStates 
 
 
-def PDLSendStates {σ : Nat} (M : AutomaticallyGeneratedModel σ) (wIndex : Nat) (i : Agent) (j : Agent) (m : Message σ) (relation : List $ (Agent × Agent × Message σ × List Nat)) : List Nat := 
+def PDLSendStates {σ : Nat} (_ : AutomaticallyGeneratedModel σ) (wIndex : Nat) (i : Agent) (j : Agent) (m : Message σ) (relation : List $ (Agent × Agent × Message σ × List Nat)) : List Nat := 
   let agentRelation : List $ List Nat := ((relation.filter (fun (agi, agj, msg, _) => agi == i && agj == j && msg == m)).map (fun (_, _, _, y) => y)).filter (fun list => list.getAtIndex! 0 0 == wIndex)
   let accessibleStates : List Nat := agentRelation.map (fun list => list.getAtIndex! 1 0)
   accessibleStates 
 
-def PDLRecvStates {σ : Nat} (M : AutomaticallyGeneratedModel σ) (wIndex : Nat) (j : Agent) (m : Message σ) (relation : List $ (Agent × Message σ × List Nat)) : List Nat :=
+def PDLRecvStates {σ : Nat} (_ : AutomaticallyGeneratedModel σ) (wIndex : Nat) (j : Agent) (m : Message σ) (relation : List $ (Agent × Message σ × List Nat)) : List Nat :=
+  let agentRelation : List $ List Nat := ((relation.filter (fun (agj, msg, _) => agj == j && msg == m)).map (fun (_, _, y) => y)).filter (fun list => list.getAtIndex! 0 0 == wIndex)
+  let accessibleStates : List Nat := agentRelation.map (fun list => list.getAtIndex! 1 0)
+  accessibleStates 
+
+def PDLGenStates {σ : Nat} (_ : AutomaticallyGeneratedModel σ) (wIndex : Nat) (j : Agent) (m : Message σ) (relation : List $ (Agent × Message σ × List Nat)) : List Nat :=
   let agentRelation : List $ List Nat := ((relation.filter (fun (agj, msg, _) => agj == j && msg == m)).map (fun (_, _, y) => y)).filter (fun list => list.getAtIndex! 0 0 == wIndex)
   let accessibleStates : List Nat := agentRelation.map (fun list => list.getAtIndex! 1 0)
   accessibleStates 
@@ -313,9 +586,11 @@ def PDLRecvStates {σ : Nat} (M : AutomaticallyGeneratedModel σ) (wIndex : Nat)
 def SatisfiesAtState {σ : Nat} (M : AutomaticallyGeneratedModel σ) (φ : Formula σ) (wIndex : Nat) : Bool :=
   match φ with
   | Formula.atom _ => True 
-  | φ ⊃ ψ => (SatisfiesAtState M φ wIndex) → (SatisfiesAtState M ψ wIndex)
+  | Formula.true => True 
+  | φ implies ψ => (SatisfiesAtState M φ wIndex) → (SatisfiesAtState M ψ wIndex)
   | ~φ => !(SatisfiesAtState M φ wIndex) 
   | 𝕏 agent, m => AwarenessSatisfies M wIndex agent m  
+  | Δ agent, m => AwarenessSatisfies M wIndex agent m 
   | 𝔹 agent, φ => 
     let accessibleStates := ModalKBStates M wIndex agent M.R𝔹
     let applySatisfaction := accessibleStates.map (fun accessibleState => SatisfiesAtState M φ accessibleState)
@@ -326,6 +601,10 @@ def SatisfiesAtState {σ : Nat} (M : AutomaticallyGeneratedModel σ) (φ : Formu
     applySatisfaction.foldr (fun x y => x && y) True 
   | [recv j(m)] φ => 
     let accessibleStates := PDLRecvStates M wIndex j m M.RPDLRecv 
+    let applySatisfaction := accessibleStates.map (fun accessibleState => SatisfiesAtState M φ accessibleState)
+    applySatisfaction.foldr (fun x y => x && y) True 
+  | [gen i(m)] φ => 
+    let accessibleStates := PDLGenStates M wIndex i m M.RPDLGen
     let applySatisfaction := accessibleStates.map (fun accessibleState => SatisfiesAtState M φ accessibleState)
     applySatisfaction.foldr (fun x y => x && y) True 
 
@@ -443,7 +722,7 @@ def BuildModel {σ : Nat} (P : Protocol σ) : AutomaticallyGeneratedModel σ :=
     if agentPos == initialAgentPosition then ik.append [initialAction.Message] else ik.append []))
 
   let agentsInitialKnowledgeKeys := (agentsInitialKnowledge.zip (List.range agentsNumber)).map (fun (ik, pos) => 
-    let agentByPos := ((agentsPositions.filter (fun ((x : Agent), y) => y == pos)).map (fun ((x : Agent), (_ : Nat)) => x)).getAtIndex! 0 ""
+    let agentByPos := ((agentsPositions.filter (fun ((_ : Agent), y) => y == pos)).map (fun ((x : Agent), (_ : Nat)) => x)).getAtIndex! 0 ""
     let searchInSymmetricKeys := P.SymmetricKeys.filter (fun ((x : Agent), (y : Agent), (_ : Message σ)) => x == agentByPos || y == agentByPos)
     let key := if searchInSymmetricKeys.length > 0 then (searchInSymmetricKeys.getAtIndex! 0 (("", "", Message.empty) : Agent × Agent × Message σ)).snd.snd else Message.empty 
     let otherAgentsPublicKeys : List $ Message σ := (P.Agents.filter (fun ag => ag != agentByPos)).map (fun ag => pk(ag))
@@ -489,6 +768,7 @@ def BuildModel {σ : Nat} (P : Protocol σ) : AutomaticallyGeneratedModel σ :=
     R𝔹 := belief,
     RPDLSend := pdlRelationSend,
     RPDLRecv := result.snd.snd,
+    RPDLGen := [],
   }
 
 /-
